sumDecode defined

src/codec.v
@@ -2,37 +2,43 @@ Require Import ast_instructions.
 Require Import association_list.
 Require Import binary.
   
+Variable A B : Type.
   
 (* Simple encoder for unit *)
 Definition unitEncode (l: list bool) : (unit*list bool) :=
   (tt, l).
 
 (* Product decoding function in order to decode 2 kinds of data. eg: (Opcode * arguments) *)
-Fixpoint crossDecode (A B: Type) (l: list bool) (dA: list bool -> (A*list bool)) (dB: list bool -> (B*list bool)) : (A*B*list bool) :=
+Fixpoint crossDecode (l: list bool) (dA: list bool -> (option A*list bool)) (dB: list bool -> (option B*list bool)) : (option A*option B*list bool) :=
   match dA l with
   | (a, l') => match dB l' with
                | (b, l'') => (a,b,l'')
                end
   end.
-
+  
 (* Decoding function using 2 given codecs *)
-Fixpoint sumDecode (A B: Type) (l: list bool) (dA: list bool -> (A*list bool)) (dB: list bool -> (B*list bool)) : (A*B*list bool) :=
+Fixpoint sumDecode (l: list bool) (dA: list bool -> (option A*list bool)) (dB: list bool -> (option B*list bool)) : ((option A + option B)*list bool) :=
   match dA l with
+  | (None, l') => match dB l' with
+             | (b, l'') => ((inr b),l'')
+             end
+  | (a, l') => ((inl a),l')
+  end.
 
-
-(* Returns the decoded result from a decoding function *)
-Fixpoint getResultDecode (A: Type) (l: list bool) (decode: list bool -> (A*list bool)) : A :=
+(* Returns the decoded result from a decoding function. Is it useful ? *)
+Fixpoint getResultDecode (l: list bool) (decode: list bool -> (A*list bool)) : A :=
   match decode l with
   | (a, l') => a
   end.
 
-(* Returns the remainding list from a decoding function *)
-Fixpoint getRemListDecode (A: Type) (l: list bool) (decode: list bool -> (A*list bool)) : list bool :=
+(* Returns the remainding list from a decoding function. Is it useful ?  *)
+Fixpoint getRemListDecode (l: list bool) (decode: list bool -> (A*list bool)) : list bool :=
   match decode l with
   | (a, l') => l'
   end.
 
 (* We want to prove the correctness of the decoding function *) 
-(* Lemma decode_composition : forall (A B: Type) (l: list bool) (dA: list bool -> (A*list bool)) (dB: list bool -> (B*list bool)),
-    . *)
-    
+Lemma decode_composition : forall (l l' l'': list bool) (a: A) (b: B) (dA: list bool -> (A*list bool)) (dB: list (* bool -> (B*list bool)),
+  crossDecode l dA dB = (a, b, l'') -> dA l = (a, l') /\ dB l' = (b, l'').
+Proof. *)
+  
